challenge_response.v
@@ -1,6 +1,6 @@
 From stdpp Require Import base gmap.
 From mathcomp Require Import ssreflect.
-From iris.algebra Require Import agree auth csum gset gmap excl namespace_map frac.
+From iris.algebra Require Import agree auth csum gset gmap excl frac.
 From iris.heap_lang Require Import notation proofmode.
 From cryptis Require Import lib term cryptis primitives tactics session.
 
@@ -19,7 +19,7 @@ A --> B: {nA, nB, vk(B)}_sk(A)
 
 Section CR.
 
-Context `{!heapG Σ, !cryptisG Σ, !sessionG Σ}.
+Context `{!heapGS Σ, !cryptisG Σ, !sessionG Σ}.
 Notation iProp := (iProp Σ).
 
 Implicit Types t : term.
