dh.v
@@ -1,7 +1,7 @@
 From stdpp Require Import base gmap.
 From mathcomp Require Import ssreflect.
 From stdpp Require Import namespaces.
-From iris.algebra Require Import agree auth csum gset gmap excl namespace_map frac.
+From iris.algebra Require Import agree auth csum gset gmap excl frac.
 From iris.heap_lang Require Import notation proofmode.
 From cryptis Require Import lib term cryptis primitives tactics session.
 
@@ -11,7 +11,7 @@ Unset Printing Implicit Defensive.
 
 Section DH.
 
-Context `{!cryptisG Σ, !heapG Σ}.
+Context `{!cryptisG Σ, !heapGS Σ}.
 Notation iProp := (iProp Σ).
 
 Implicit Types t : term.
@@ -50,7 +50,7 @@ iDestruct "p_t" as "(_ & _ & [contra | p_t])".
 iDestruct "aP" as "(_ & _ & #aP)".
 iSpecialize ("aP" with "p_t"); iModIntro.
 iDestruct "aP" as (g' a') "# [%e aP]".
-by case/TExp_inj: e => _ /Permutation_singleton [] ->; eauto.
+by case/TExp_inj: e => _ /Permutation_singleton_r [] ->; eauto.
 Qed.
 
 Lemma dh_seed_elim2 g a t :
@@ -102,7 +102,7 @@ Next Obligation.
 iIntros (L ?? t x N E sub).
 iDestruct 1 as (g a) "[-> token]".
 iDestruct 1 as (??)  "[%e  meta]".
-move/TExp_inj: e => [_ /Permutation_singleton [<-]].
+move/TExp_inj: e => [_ /Permutation_singleton_r [<-]].
 by iApply (term_meta_meta_token with "token meta").
 Qed.
 
@@ -110,7 +110,7 @@ Next Obligation.
 iIntros (L ?? t N x1 x2).
 iDestruct 1 as (g a) "[-> meta1]".
 iDestruct 1 as (??)  "[%e meta2]".
-move/TExp_inj: e => [_ /Permutation_singleton [<-]].
+move/TExp_inj: e => [_ /Permutation_singleton_r [<-]].
 by iApply (term_meta_agree with "meta1 meta2").
 Qed.
 
@@ -123,7 +123,7 @@ move=> t E1 E2 sub; iSplit.
 - iDestruct 1 as "[token1 token2]".
   iDestruct "token1" as (g a) "[-> token1]".
   iDestruct "token2" as (??) "[%e token2]".
-  move/TExp_inj: e => [_ /Permutation_singleton [<-]].
+  move/TExp_inj: e => [_ /Permutation_singleton_r [<-]].
   iExists _, _; iSplit => //.
   rewrite (term_meta_token_difference _ E1 E2) //.
   by iSplitL "token1".
