primitives/notations.v
@@ -1,7 +1,7 @@
 From mathcomp Require Import ssreflect.
 From mathcomp Require order.
 From stdpp Require Import gmap.
-From iris.algebra Require Import agree auth gset gmap namespace_map.
+From iris.algebra Require Import agree auth gset gmap.
 From iris.base_logic.lib Require Import invariants.
 From iris.heap_lang Require Import notation proofmode.
 
