session.v
@@ -26,7 +26,7 @@ obtain B's resource.  The file nsl.v contains an example of this idiom.
 
 From stdpp Require Import base gmap.
 From mathcomp Require Import ssreflect.
-From iris.algebra Require Import agree auth csum gset gmap excl namespace_map frac.
+From iris.algebra Require Import agree auth csum gset gmap excl frac.
 From iris.base_logic.lib Require Import invariants.
 From iris.heap_lang Require Import notation proofmode.
 From cryptis Require Import lib term cryptis.
@@ -37,7 +37,7 @@ Unset Printing Implicit Defensive.
 
 Section Session.
 
-Context `{!cryptisG Σ, !heapG Σ}.
+Context `{!cryptisG Σ, !heapGS Σ}.
 Notation iProp  := (iProp Σ).
 Notation iPropI := (iPropI Σ).
 
